language/move-prover/bytecode-to-boogie/tests/goldenfiles/test-lib.bpl
@@ -133,12 +133,14 @@ requires ExistsTxnSenderAccount(__m, __txn);
     assume !__abort_flag;
     __saved_m := __m;
     __frame := __local_counter;
-    __local_counter := __local_counter + 7;
 
     // process and type check arguments
     assume is#Vector(gas_schedule);
     __m := UpdateLocal(__m, __frame + 0, gas_schedule);
     assume $DebugTrackLocal(6, 0, 0, 1239, gas_schedule);
+
+    // increase the local counter
+    __local_counter := __local_counter + 7;
 
     // bytecode translation starts here
     call __tmp := GetTxnSenderAddress();
@@ -204,9 +206,11 @@ requires ExistsTxnSenderAccount(__m, __txn);
     assume !__abort_flag;
     __saved_m := __m;
     __frame := __local_counter;
-    __local_counter := __local_counter + 8;
 
     // process and type check arguments
+
+    // increase the local counter
+    __local_counter := __local_counter + 8;
 
     // bytecode translation starts here
     call __tmp := LdAddr(173345816);
@@ -278,9 +282,11 @@ requires ExistsTxnSenderAccount(__m, __txn);
     assume !__abort_flag;
     __saved_m := __m;
     __frame := __local_counter;
-    __local_counter := __local_counter + 8;
 
     // process and type check arguments
+
+    // increase the local counter
+    __local_counter := __local_counter + 8;
 
     // bytecode translation starts here
     call __tmp := LdAddr(173345816);
@@ -417,12 +423,14 @@ requires ExistsTxnSenderAccount(__m, __txn);
     assume !__abort_flag;
     __saved_m := __m;
     __frame := __local_counter;
-    __local_counter := __local_counter + 3;
 
     // process and type check arguments
     assume is#Address(addr);
     __m := UpdateLocal(__m, __frame + 0, addr);
     assume $DebugTrackLocal(7, 0, 0, 645, addr);
+
+    // increase the local counter
+    __local_counter := __local_counter + 3;
 
     // bytecode translation starts here
     call __tmp := CopyOrMoveValue(GetLocal(__m, __frame + 0));
@@ -465,12 +473,14 @@ requires ExistsTxnSenderAccount(__m, __txn);
     assume !__abort_flag;
     __saved_m := __m;
     __frame := __local_counter;
-    __local_counter := __local_counter + 7;
 
     // process and type check arguments
     assume is#Address(addr);
     __m := UpdateLocal(__m, __frame + 0, addr);
     assume $DebugTrackLocal(7, 1, 0, 907, addr);
+
+    // increase the local counter
+    __local_counter := __local_counter + 7;
 
     // bytecode translation starts here
     call __tmp := CopyOrMoveValue(GetLocal(__m, __frame + 0));
@@ -525,13 +535,15 @@ requires ExistsTxnSenderAccount(__m, __txn);
     assume !__abort_flag;
     __saved_m := __m;
     __frame := __local_counter;
-    __local_counter := __local_counter + 4;
 
     // process and type check arguments
     assume is#Vector(Dereference(__m, config_ref));
-    assume IsValidReferenceParameter(__m, __frame, config_ref);
+    assume IsValidReferenceParameter(__m, __local_counter, config_ref);
     assume is#Vector(Dereference(__m, config_ref));
     assume $DebugTrackLocal(7, 2, 0, 1129, Dereference(__m, config_ref));
+
+    // increase the local counter
+    __local_counter := __local_counter + 4;
 
     // bytecode translation starts here
     call __t1 := CopyOrMoveRef(config_ref);
@@ -573,13 +585,15 @@ requires ExistsTxnSenderAccount(__m, __txn);
     assume !__abort_flag;
     __saved_m := __m;
     __frame := __local_counter;
-    __local_counter := __local_counter + 4;
 
     // process and type check arguments
     assume is#Vector(Dereference(__m, config_ref));
-    assume IsValidReferenceParameter(__m, __frame, config_ref);
+    assume IsValidReferenceParameter(__m, __local_counter, config_ref);
     assume is#Vector(Dereference(__m, config_ref));
     assume $DebugTrackLocal(7, 3, 0, 1315, Dereference(__m, config_ref));
+
+    // increase the local counter
+    __local_counter := __local_counter + 4;
 
     // bytecode translation starts here
     call __t1 := CopyOrMoveRef(config_ref);
@@ -621,13 +635,15 @@ requires ExistsTxnSenderAccount(__m, __txn);
     assume !__abort_flag;
     __saved_m := __m;
     __frame := __local_counter;
-    __local_counter := __local_counter + 4;
 
     // process and type check arguments
     assume is#Vector(Dereference(__m, config_ref));
-    assume IsValidReferenceParameter(__m, __frame, config_ref);
+    assume IsValidReferenceParameter(__m, __local_counter, config_ref);
     assume is#Vector(Dereference(__m, config_ref));
     assume $DebugTrackLocal(7, 4, 0, 1534, Dereference(__m, config_ref));
+
+    // increase the local counter
+    __local_counter := __local_counter + 4;
 
     // bytecode translation starts here
     call __t1 := CopyOrMoveRef(config_ref);
@@ -669,13 +685,15 @@ requires ExistsTxnSenderAccount(__m, __txn);
     assume !__abort_flag;
     __saved_m := __m;
     __frame := __local_counter;
-    __local_counter := __local_counter + 4;
 
     // process and type check arguments
     assume is#Vector(Dereference(__m, config_ref));
-    assume IsValidReferenceParameter(__m, __frame, config_ref);
+    assume IsValidReferenceParameter(__m, __local_counter, config_ref);
     assume is#Vector(Dereference(__m, config_ref));
     assume $DebugTrackLocal(7, 5, 0, 1747, Dereference(__m, config_ref));
+
+    // increase the local counter
+    __local_counter := __local_counter + 4;
 
     // bytecode translation starts here
     call __t1 := CopyOrMoveRef(config_ref);
@@ -717,13 +735,15 @@ requires ExistsTxnSenderAccount(__m, __txn);
     assume !__abort_flag;
     __saved_m := __m;
     __frame := __local_counter;
-    __local_counter := __local_counter + 4;
 
     // process and type check arguments
     assume is#Vector(Dereference(__m, config_ref));
-    assume IsValidReferenceParameter(__m, __frame, config_ref);
+    assume IsValidReferenceParameter(__m, __local_counter, config_ref);
     assume is#Vector(Dereference(__m, config_ref));
     assume $DebugTrackLocal(7, 6, 0, 1952, Dereference(__m, config_ref));
+
+    // increase the local counter
+    __local_counter := __local_counter + 4;
 
     // bytecode translation starts here
     call __t1 := CopyOrMoveRef(config_ref);
@@ -765,13 +785,15 @@ requires ExistsTxnSenderAccount(__m, __txn);
     assume !__abort_flag;
     __saved_m := __m;
     __frame := __local_counter;
-    __local_counter := __local_counter + 4;
 
     // process and type check arguments
     assume is#Vector(Dereference(__m, config_ref));
-    assume IsValidReferenceParameter(__m, __frame, config_ref);
+    assume IsValidReferenceParameter(__m, __local_counter, config_ref);
     assume is#Vector(Dereference(__m, config_ref));
     assume $DebugTrackLocal(7, 7, 0, 2165, Dereference(__m, config_ref));
+
+    // increase the local counter
+    __local_counter := __local_counter + 4;
 
     // bytecode translation starts here
     call __t1 := CopyOrMoveRef(config_ref);
@@ -818,7 +840,6 @@ requires ExistsTxnSenderAccount(__m, __txn);
     assume !__abort_flag;
     __saved_m := __m;
     __frame := __local_counter;
-    __local_counter := __local_counter + 14;
 
     // process and type check arguments
     assume is#ByteArray(consensus_pubkey);
@@ -839,6 +860,9 @@ requires ExistsTxnSenderAccount(__m, __txn);
     assume is#ByteArray(fullnodes_network_address);
     __m := UpdateLocal(__m, __frame + 5, fullnodes_network_address);
     assume $DebugTrackLocal(7, 8, 5, 2532, fullnodes_network_address);
+
+    // increase the local counter
+    __local_counter := __local_counter + 14;
 
     // bytecode translation starts here
     call __tmp := CopyOrMoveValue(GetLocal(__m, __frame + 0));
@@ -907,12 +931,14 @@ requires ExistsTxnSenderAccount(__m, __txn);
     assume !__abort_flag;
     __saved_m := __m;
     __frame := __local_counter;
-    __local_counter := __local_counter + 12;
 
     // process and type check arguments
     assume is#ByteArray(consensus_pubkey);
     __m := UpdateLocal(__m, __frame + 0, consensus_pubkey);
     assume $DebugTrackLocal(7, 9, 0, 3648, consensus_pubkey);
+
+    // increase the local counter
+    __local_counter := __local_counter + 12;
 
     // bytecode translation starts here
     call __tmp := GetTxnSenderAddress();
@@ -987,12 +1013,14 @@ requires ExistsTxnSenderAccount(__m, __txn);
     assume !__abort_flag;
     __saved_m := __m;
     __frame := __local_counter;
-    __local_counter := __local_counter + 12;
 
     // process and type check arguments
     assume is#ByteArray(validator_network_identity_pubkey);
     __m := UpdateLocal(__m, __frame + 0, validator_network_identity_pubkey);
     assume $DebugTrackLocal(7, 10, 0, 4265, validator_network_identity_pubkey);
+
+    // increase the local counter
+    __local_counter := __local_counter + 12;
 
     // bytecode translation starts here
     call __tmp := GetTxnSenderAddress();
@@ -1067,12 +1095,14 @@ requires ExistsTxnSenderAccount(__m, __txn);
     assume !__abort_flag;
     __saved_m := __m;
     __frame := __local_counter;
-    __local_counter := __local_counter + 12;
 
     // process and type check arguments
     assume is#ByteArray(validator_network_address);
     __m := UpdateLocal(__m, __frame + 0, validator_network_address);
     assume $DebugTrackLocal(7, 11, 0, 4890, validator_network_address);
+
+    // increase the local counter
+    __local_counter := __local_counter + 12;
 
     // bytecode translation starts here
     call __tmp := GetTxnSenderAddress();
@@ -1205,12 +1235,14 @@ requires ExistsTxnSenderAccount(__m, __txn);
     assume !__abort_flag;
     __saved_m := __m;
     __frame := __local_counter;
-    __local_counter := __local_counter + 5;
 
     // process and type check arguments
     assume IsValidU64(amount);
     __m := UpdateLocal(__m, __frame + 0, amount);
     assume $DebugTrackLocal(8, 0, 0, 807, amount);
+
+    // increase the local counter
+    __local_counter := __local_counter + 5;
 
     // bytecode translation starts here
     call __tmp := CopyOrMoveValue(GetLocal(__m, __frame + 0));
@@ -1281,16 +1313,18 @@ requires ExistsTxnSenderAccount(__m, __txn);
     assume !__abort_flag;
     __saved_m := __m;
     __frame := __local_counter;
-    __local_counter := __local_counter + 21;
 
     // process and type check arguments
     assume IsValidU64(value);
     __m := UpdateLocal(__m, __frame + 0, value);
     assume $DebugTrackLocal(8, 1, 0, 1231, value);
     assume is#Vector(Dereference(__m, capability));
-    assume IsValidReferenceParameter(__m, __frame, capability);
+    assume IsValidReferenceParameter(__m, __local_counter, capability);
     assume is#Vector(Dereference(__m, capability));
     assume $DebugTrackLocal(8, 1, 1, 1231, Dereference(__m, capability));
+
+    // increase the local counter
+    __local_counter := __local_counter + 21;
 
     // bytecode translation starts here
     call __tmp := CopyOrMoveValue(GetLocal(__m, __frame + 0));
@@ -1409,9 +1443,11 @@ requires ExistsTxnSenderAccount(__m, __txn);
     assume !__abort_flag;
     __saved_m := __m;
     __frame := __local_counter;
-    __local_counter := __local_counter + 9;
 
     // process and type check arguments
+
+    // increase the local counter
+    __local_counter := __local_counter + 9;
 
     // bytecode translation starts here
     call __tmp := GetTxnSenderAddress();
@@ -1488,9 +1524,11 @@ requires ExistsTxnSenderAccount(__m, __txn);
     assume !__abort_flag;
     __saved_m := __m;
     __frame := __local_counter;
-    __local_counter := __local_counter + 4;
 
     // process and type check arguments
+
+    // increase the local counter
+    __local_counter := __local_counter + 4;
 
     // bytecode translation starts here
     call __tmp := LdAddr(173345816);
@@ -1538,9 +1576,11 @@ requires ExistsTxnSenderAccount(__m, __txn);
     assume !__abort_flag;
     __saved_m := __m;
     __frame := __local_counter;
-    __local_counter := __local_counter + 2;
 
     // process and type check arguments
+
+    // increase the local counter
+    __local_counter := __local_counter + 2;
 
     // bytecode translation starts here
     call __tmp := LdConst(0);
@@ -1580,13 +1620,15 @@ requires ExistsTxnSenderAccount(__m, __txn);
     assume !__abort_flag;
     __saved_m := __m;
     __frame := __local_counter;
-    __local_counter := __local_counter + 4;
 
     // process and type check arguments
     assume is#Vector(Dereference(__m, coin_ref));
-    assume IsValidReferenceParameter(__m, __frame, coin_ref);
+    assume IsValidReferenceParameter(__m, __local_counter, coin_ref);
     assume is#Vector(Dereference(__m, coin_ref));
     assume $DebugTrackLocal(8, 5, 0, 2888, Dereference(__m, coin_ref));
+
+    // increase the local counter
+    __local_counter := __local_counter + 4;
 
     // bytecode translation starts here
     call __t1 := CopyOrMoveRef(coin_ref);
@@ -1631,7 +1673,6 @@ requires ExistsTxnSenderAccount(__m, __txn);
     assume !__abort_flag;
     __saved_m := __m;
     __frame := __local_counter;
-    __local_counter := __local_counter + 8;
 
     // process and type check arguments
     assume is#Vector(coin);
@@ -1640,6 +1681,9 @@ requires ExistsTxnSenderAccount(__m, __txn);
     assume IsValidU64(amount);
     __m := UpdateLocal(__m, __frame + 1, amount);
     assume $DebugTrackLocal(8, 6, 1, 3109, amount);
+
+    // increase the local counter
+    __local_counter := __local_counter + 8;
 
     // bytecode translation starts here
     call __t3 := BorrowLoc(__frame + 0);
@@ -1714,16 +1758,18 @@ requires ExistsTxnSenderAccount(__m, __txn);
     assume !__abort_flag;
     __saved_m := __m;
     __frame := __local_counter;
-    __local_counter := __local_counter + 18;
 
     // process and type check arguments
     assume is#Vector(Dereference(__m, coin_ref));
-    assume IsValidReferenceParameter(__m, __frame, coin_ref);
+    assume IsValidReferenceParameter(__m, __local_counter, coin_ref);
     assume is#Vector(Dereference(__m, coin_ref));
     assume $DebugTrackLocal(8, 7, 0, 3557, Dereference(__m, coin_ref));
     assume IsValidU64(amount);
     __m := UpdateLocal(__m, __frame + 1, amount);
     assume $DebugTrackLocal(8, 7, 1, 3557, amount);
+
+    // increase the local counter
+    __local_counter := __local_counter + 18;
 
     // bytecode translation starts here
     call __t3 := CopyOrMoveRef(coin_ref);
@@ -1815,7 +1861,6 @@ requires ExistsTxnSenderAccount(__m, __txn);
     assume !__abort_flag;
     __saved_m := __m;
     __frame := __local_counter;
-    __local_counter := __local_counter + 5;
 
     // process and type check arguments
     assume is#Vector(coin1);
@@ -1824,6 +1869,9 @@ requires ExistsTxnSenderAccount(__m, __txn);
     assume is#Vector(coin2);
     __m := UpdateLocal(__m, __frame + 1, coin2);
     assume $DebugTrackLocal(8, 8, 1, 4041, coin2);
+
+    // increase the local counter
+    __local_counter := __local_counter + 5;
 
     // bytecode translation starts here
     call __t2 := BorrowLoc(__frame + 0);
@@ -1881,16 +1929,18 @@ requires ExistsTxnSenderAccount(__m, __txn);
     assume !__abort_flag;
     __saved_m := __m;
     __frame := __local_counter;
-    __local_counter := __local_counter + 14;
 
     // process and type check arguments
     assume is#Vector(Dereference(__m, coin_ref));
-    assume IsValidReferenceParameter(__m, __frame, coin_ref);
+    assume IsValidReferenceParameter(__m, __local_counter, coin_ref);
     assume is#Vector(Dereference(__m, coin_ref));
     assume $DebugTrackLocal(8, 9, 0, 4352, Dereference(__m, coin_ref));
     assume is#Vector(check);
     __m := UpdateLocal(__m, __frame + 1, check);
     assume $DebugTrackLocal(8, 9, 1, 4352, check);
+
+    // increase the local counter
+    __local_counter := __local_counter + 14;
 
     // bytecode translation starts here
     call __t4 := CopyOrMoveRef(coin_ref);
@@ -1967,12 +2017,14 @@ requires ExistsTxnSenderAccount(__m, __txn);
     assume !__abort_flag;
     __saved_m := __m;
     __frame := __local_counter;
-    __local_counter := __local_counter + 9;
 
     // process and type check arguments
     assume is#Vector(coin);
     __m := UpdateLocal(__m, __frame + 0, coin);
     assume $DebugTrackLocal(8, 10, 0, 4858, coin);
+
+    // increase the local counter
+    __local_counter := __local_counter + 9;
 
     // bytecode translation starts here
     call __tmp := CopyOrMoveValue(GetLocal(__m, __frame + 0));
@@ -2067,9 +2119,11 @@ requires ExistsTxnSenderAccount(__m, __txn);
     assume !__abort_flag;
     __saved_m := __m;
     __frame := __local_counter;
-    __local_counter := __local_counter + 9;
 
     // process and type check arguments
+
+    // increase the local counter
+    __local_counter := __local_counter + 9;
 
     // bytecode translation starts here
     call __tmp := GetTxnSenderAddress();
@@ -2160,7 +2214,6 @@ requires ExistsTxnSenderAccount(__m, __txn);
     assume !__abort_flag;
     __saved_m := __m;
     __frame := __local_counter;
-    __local_counter := __local_counter + 25;
 
     // process and type check arguments
     assume is#Address(proposer);
@@ -2169,6 +2222,9 @@ requires ExistsTxnSenderAccount(__m, __txn);
     assume IsValidU64(timestamp);
     __m := UpdateLocal(__m, __frame + 1, timestamp);
     assume $DebugTrackLocal(9, 1, 1, 743, timestamp);
+
+    // increase the local counter
+    __local_counter := __local_counter + 25;
 
     // bytecode translation starts here
     call __tmp := LdAddr(173345816);
@@ -2289,9 +2345,11 @@ requires ExistsTxnSenderAccount(__m, __txn);
     assume !__abort_flag;
     __saved_m := __m;
     __frame := __local_counter;
-    __local_counter := __local_counter + 4;
 
     // process and type check arguments
+
+    // increase the local counter
+    __local_counter := __local_counter + 4;
 
     // bytecode translation starts here
     call __tmp := LdAddr(173345816);
@@ -2373,9 +2431,11 @@ requires ExistsTxnSenderAccount(__m, __txn);
     assume !__abort_flag;
     __saved_m := __m;
     __frame := __local_counter;
-    __local_counter := __local_counter + 9;
 
     // process and type check arguments
+
+    // increase the local counter
+    __local_counter := __local_counter + 9;
 
     // bytecode translation starts here
     call __tmp := GetTxnSenderAddress();
@@ -2454,12 +2514,14 @@ requires ExistsTxnSenderAccount(__m, __txn);
     assume !__abort_flag;
     __saved_m := __m;
     __frame := __local_counter;
-    __local_counter := __local_counter + 12;
 
     // process and type check arguments
     assume IsValidU64(new_duration);
     __m := UpdateLocal(__m, __frame + 0, new_duration);
     assume $DebugTrackLocal(10, 1, 0, 564, new_duration);
+
+    // increase the local counter
+    __local_counter := __local_counter + 12;
 
     // bytecode translation starts here
     call __tmp := GetTxnSenderAddress();
@@ -2552,12 +2614,14 @@ requires ExistsTxnSenderAccount(__m, __txn);
     assume !__abort_flag;
     __saved_m := __m;
     __frame := __local_counter;
-    __local_counter := __local_counter + 23;
 
     // process and type check arguments
     assume IsValidU64(timestamp);
     __m := UpdateLocal(__m, __frame + 0, timestamp);
     assume $DebugTrackLocal(10, 2, 0, 911, timestamp);
+
+    // increase the local counter
+    __local_counter := __local_counter + 23;
 
     // bytecode translation starts here
     call __tmp := CopyOrMoveValue(GetLocal(__m, __frame + 0));
@@ -2885,7 +2949,6 @@ requires ExistsTxnSenderAccount(__m, __txn);
     assume !__abort_flag;
     __saved_m := __m;
     __frame := __local_counter;
-    __local_counter := __local_counter + 5;
 
     // process and type check arguments
     assume is#Address(payee);
@@ -2894,6 +2957,9 @@ requires ExistsTxnSenderAccount(__m, __txn);
     assume is#Vector(to_deposit);
     __m := UpdateLocal(__m, __frame + 1, to_deposit);
     assume $DebugTrackLocal(11, 0, 1, 3305, to_deposit);
+
+    // increase the local counter
+    __local_counter := __local_counter + 5;
 
     // bytecode translation starts here
     call __tmp := CopyOrMoveValue(GetLocal(__m, __frame + 0));
@@ -2939,7 +3005,6 @@ requires ExistsTxnSenderAccount(__m, __txn);
     assume !__abort_flag;
     __saved_m := __m;
     __frame := __local_counter;
-    __local_counter := __local_counter + 7;
 
     // process and type check arguments
     assume is#Address(payee);
@@ -2951,6 +3016,9 @@ requires ExistsTxnSenderAccount(__m, __txn);
     assume is#ByteArray(metadata);
     __m := UpdateLocal(__m, __frame + 2, metadata);
     assume $DebugTrackLocal(11, 1, 2, 3567, metadata);
+
+    // increase the local counter
+    __local_counter := __local_counter + 7;
 
     // bytecode translation starts here
     call __tmp := CopyOrMoveValue(GetLocal(__m, __frame + 0));
@@ -3025,7 +3093,6 @@ requires ExistsTxnSenderAccount(__m, __txn);
     assume !__abort_flag;
     __saved_m := __m;
     __frame := __local_counter;
-    __local_counter := __local_counter + 33;
 
     // process and type check arguments
     assume is#Address(payee);
@@ -3040,6 +3107,9 @@ requires ExistsTxnSenderAccount(__m, __txn);
     assume is#ByteArray(metadata);
     __m := UpdateLocal(__m, __frame + 3, metadata);
     assume $DebugTrackLocal(11, 2, 3, 4018, metadata);
+
+    // increase the local counter
+    __local_counter := __local_counter + 33;
 
     // bytecode translation starts here
     call __t7 := BorrowLoc(__frame + 2);
@@ -3193,7 +3263,6 @@ requires ExistsTxnSenderAccount(__m, __txn);
     assume !__abort_flag;
     __saved_m := __m;
     __frame := __local_counter;
-    __local_counter := __local_counter + 9;
 
     // process and type check arguments
     assume is#Address(payee);
@@ -3202,6 +3271,9 @@ requires ExistsTxnSenderAccount(__m, __txn);
     assume IsValidU64(amount);
     __m := UpdateLocal(__m, __frame + 1, amount);
     assume $DebugTrackLocal(11, 3, 1, 5776, amount);
+
+    // increase the local counter
+    __local_counter := __local_counter + 9;
 
     // bytecode translation starts here
     call __tmp := CopyOrMoveValue(GetLocal(__m, __frame + 0));
@@ -3278,16 +3350,18 @@ requires ExistsTxnSenderAccount(__m, __txn);
     assume !__abort_flag;
     __saved_m := __m;
     __frame := __local_counter;
-    __local_counter := __local_counter + 8;
 
     // process and type check arguments
     assume is#Vector(Dereference(__m, account));
-    assume IsValidReferenceParameter(__m, __frame, account);
+    assume IsValidReferenceParameter(__m, __local_counter, account);
     assume is#Vector(Dereference(__m, account));
     assume $DebugTrackLocal(11, 4, 0, 6237, Dereference(__m, account));
     assume IsValidU64(amount);
     __m := UpdateLocal(__m, __frame + 1, amount);
     assume $DebugTrackLocal(11, 4, 1, 6237, amount);
+
+    // increase the local counter
+    __local_counter := __local_counter + 8;
 
     // bytecode translation starts here
     call __t3 := CopyOrMoveRef(account);
@@ -3351,12 +3425,14 @@ requires ExistsTxnSenderAccount(__m, __txn);
     assume !__abort_flag;
     __saved_m := __m;
     __frame := __local_counter;
-    __local_counter := __local_counter + 11;
 
     // process and type check arguments
     assume IsValidU64(amount);
     __m := UpdateLocal(__m, __frame + 0, amount);
     assume $DebugTrackLocal(11, 5, 0, 6552, amount);
+
+    // increase the local counter
+    __local_counter := __local_counter + 11;
 
     // bytecode translation starts here
     call __tmp := GetTxnSenderAddress();
@@ -3439,16 +3515,18 @@ requires ExistsTxnSenderAccount(__m, __txn);
     assume !__abort_flag;
     __saved_m := __m;
     __frame := __local_counter;
-    __local_counter := __local_counter + 10;
 
     // process and type check arguments
     assume is#Vector(Dereference(__m, cap));
-    assume IsValidReferenceParameter(__m, __frame, cap);
+    assume IsValidReferenceParameter(__m, __local_counter, cap);
     assume is#Vector(Dereference(__m, cap));
     assume $DebugTrackLocal(11, 6, 0, 7192, Dereference(__m, cap));
     assume IsValidU64(amount);
     __m := UpdateLocal(__m, __frame + 1, amount);
     assume $DebugTrackLocal(11, 6, 1, 7192, amount);
+
+    // increase the local counter
+    __local_counter := __local_counter + 10;
 
     // bytecode translation starts here
     call __t3 := CopyOrMoveRef(cap);
@@ -3526,9 +3604,11 @@ requires ExistsTxnSenderAccount(__m, __txn);
     assume !__abort_flag;
     __saved_m := __m;
     __frame := __local_counter;
-    __local_counter := __local_counter + 15;
 
     // process and type check arguments
+
+    // increase the local counter
+    __local_counter := __local_counter + 15;
 
     // bytecode translation starts here
     call __tmp := GetTxnSenderAddress();
@@ -3624,12 +3704,14 @@ requires ExistsTxnSenderAccount(__m, __txn);
     assume !__abort_flag;
     __saved_m := __m;
     __frame := __local_counter;
-    __local_counter := __local_counter + 10;
 
     // process and type check arguments
     assume is#Vector(cap);
     __m := UpdateLocal(__m, __frame + 0, cap);
     assume $DebugTrackLocal(11, 8, 0, 8391, cap);
+
+    // increase the local counter
+    __local_counter := __local_counter + 10;
 
     // bytecode translation starts here
     call __tmp := CopyOrMoveValue(GetLocal(__m, __frame + 0));
@@ -3701,14 +3783,13 @@ requires ExistsTxnSenderAccount(__m, __txn);
     assume !__abort_flag;
     __saved_m := __m;
     __frame := __local_counter;
-    __local_counter := __local_counter + 16;
 
     // process and type check arguments
     assume is#Address(payee);
     __m := UpdateLocal(__m, __frame + 0, payee);
     assume $DebugTrackLocal(11, 9, 0, 9236, payee);
     assume is#Vector(Dereference(__m, cap));
-    assume IsValidReferenceParameter(__m, __frame, cap);
+    assume IsValidReferenceParameter(__m, __local_counter, cap);
     assume is#Vector(Dereference(__m, cap));
     assume $DebugTrackLocal(11, 9, 1, 9236, Dereference(__m, cap));
     assume IsValidU64(amount);
@@ -3717,6 +3798,9 @@ requires ExistsTxnSenderAccount(__m, __txn);
     assume is#ByteArray(metadata);
     __m := UpdateLocal(__m, __frame + 3, metadata);
     assume $DebugTrackLocal(11, 9, 3, 9236, metadata);
+
+    // increase the local counter
+    __local_counter := __local_counter + 16;
 
     // bytecode translation starts here
     call __tmp := CopyOrMoveValue(GetLocal(__m, __frame + 0));
@@ -3808,7 +3892,6 @@ requires ExistsTxnSenderAccount(__m, __txn);
     assume !__abort_flag;
     __saved_m := __m;
     __frame := __local_counter;
-    __local_counter := __local_counter + 11;
 
     // process and type check arguments
     assume is#Address(payee);
@@ -3820,6 +3903,9 @@ requires ExistsTxnSenderAccount(__m, __txn);
     assume is#ByteArray(metadata);
     __m := UpdateLocal(__m, __frame + 2, metadata);
     assume $DebugTrackLocal(11, 10, 2, 9947, metadata);
+
+    // increase the local counter
+    __local_counter := __local_counter + 11;
 
     // bytecode translation starts here
     call __tmp := CopyOrMoveValue(GetLocal(__m, __frame + 0));
@@ -3896,7 +3982,6 @@ requires ExistsTxnSenderAccount(__m, __txn);
     assume !__abort_flag;
     __saved_m := __m;
     __frame := __local_counter;
-    __local_counter := __local_counter + 5;
 
     // process and type check arguments
     assume is#Address(payee);
@@ -3905,6 +3990,9 @@ requires ExistsTxnSenderAccount(__m, __txn);
     assume IsValidU64(amount);
     __m := UpdateLocal(__m, __frame + 1, amount);
     assume $DebugTrackLocal(11, 11, 1, 10530, amount);
+
+    // increase the local counter
+    __local_counter := __local_counter + 5;
 
     // bytecode translation starts here
     call __tmp := CopyOrMoveValue(GetLocal(__m, __frame + 0));
@@ -3949,16 +4037,18 @@ requires ExistsTxnSenderAccount(__m, __txn);
     assume !__abort_flag;
     __saved_m := __m;
     __frame := __local_counter;
-    __local_counter := __local_counter + 5;
 
     // process and type check arguments
     assume is#Vector(Dereference(__m, account));
-    assume IsValidReferenceParameter(__m, __frame, account);
+    assume IsValidReferenceParameter(__m, __local_counter, account);
     assume is#Vector(Dereference(__m, account));
     assume $DebugTrackLocal(11, 12, 0, 10698, Dereference(__m, account));
     assume is#ByteArray(new_authentication_key);
     __m := UpdateLocal(__m, __frame + 1, new_authentication_key);
     assume $DebugTrackLocal(11, 12, 1, 10698, new_authentication_key);
+
+    // increase the local counter
+    __local_counter := __local_counter + 5;
 
     // bytecode translation starts here
     call __tmp := CopyOrMoveValue(GetLocal(__m, __frame + 1));
@@ -4004,12 +4094,14 @@ requires ExistsTxnSenderAccount(__m, __txn);
     assume !__abort_flag;
     __saved_m := __m;
     __frame := __local_counter;
-    __local_counter := __local_counter + 10;
 
     // process and type check arguments
     assume is#ByteArray(new_authentication_key);
     __m := UpdateLocal(__m, __frame + 0, new_authentication_key);
     assume $DebugTrackLocal(11, 13, 0, 11025, new_authentication_key);
+
+    // increase the local counter
+    __local_counter := __local_counter + 10;
 
     // bytecode translation starts here
     call __tmp := GetTxnSenderAddress();
@@ -4083,16 +4175,18 @@ requires ExistsTxnSenderAccount(__m, __txn);
     assume !__abort_flag;
     __saved_m := __m;
     __frame := __local_counter;
-    __local_counter := __local_counter + 7;
 
     // process and type check arguments
     assume is#Vector(Dereference(__m, cap));
-    assume IsValidReferenceParameter(__m, __frame, cap);
+    assume IsValidReferenceParameter(__m, __local_counter, cap);
     assume is#Vector(Dereference(__m, cap));
     assume $DebugTrackLocal(11, 14, 0, 11765, Dereference(__m, cap));
     assume is#ByteArray(new_authentication_key);
     __m := UpdateLocal(__m, __frame + 1, new_authentication_key);
     assume $DebugTrackLocal(11, 14, 1, 11765, new_authentication_key);
+
+    // increase the local counter
+    __local_counter := __local_counter + 7;
 
     // bytecode translation starts here
     call __t2 := CopyOrMoveRef(cap);
@@ -4156,9 +4250,11 @@ requires ExistsTxnSenderAccount(__m, __txn);
     assume !__abort_flag;
     __saved_m := __m;
     __frame := __local_counter;
-    __local_counter := __local_counter + 13;
 
     // process and type check arguments
+
+    // increase the local counter
+    __local_counter := __local_counter + 13;
 
     // bytecode translation starts here
     call __tmp := GetTxnSenderAddress();
@@ -4248,12 +4344,14 @@ requires ExistsTxnSenderAccount(__m, __txn);
     assume !__abort_flag;
     __saved_m := __m;
     __frame := __local_counter;
-    __local_counter := __local_counter + 10;
 
     // process and type check arguments
     assume is#Vector(cap);
     __m := UpdateLocal(__m, __frame + 0, cap);
     assume $DebugTrackLocal(11, 16, 0, 12924, cap);
+
+    // increase the local counter
+    __local_counter := __local_counter + 10;
 
     // bytecode translation starts here
     call __tmp := CopyOrMoveValue(GetLocal(__m, __frame + 0));
@@ -4331,12 +4429,14 @@ requires ExistsTxnSenderAccount(__m, __txn);
     assume !__abort_flag;
     __saved_m := __m;
     __frame := __local_counter;
-    __local_counter := __local_counter + 19;
 
     // process and type check arguments
     assume is#Address(fresh_address);
     __m := UpdateLocal(__m, __frame + 0, fresh_address);
     assume $DebugTrackLocal(11, 17, 0, 13761, fresh_address);
+
+    // increase the local counter
+    __local_counter := __local_counter + 19;
 
     // bytecode translation starts here
     call __tmp := LdConst(0);
@@ -4455,7 +4555,6 @@ requires ExistsTxnSenderAccount(__m, __txn);
     assume !__abort_flag;
     __saved_m := __m;
     __frame := __local_counter;
-    __local_counter := __local_counter + 8;
 
     // process and type check arguments
     assume is#Address(fresh_address);
@@ -4464,6 +4563,9 @@ requires ExistsTxnSenderAccount(__m, __txn);
     assume IsValidU64(initial_balance);
     __m := UpdateLocal(__m, __frame + 1, initial_balance);
     assume $DebugTrackLocal(11, 18, 1, 14744, initial_balance);
+
+    // increase the local counter
+    __local_counter := __local_counter + 8;
 
     // bytecode translation starts here
     call __tmp := CopyOrMoveValue(GetLocal(__m, __frame + 0));
@@ -4533,13 +4635,15 @@ requires ExistsTxnSenderAccount(__m, __txn);
     assume !__abort_flag;
     __saved_m := __m;
     __frame := __local_counter;
-    __local_counter := __local_counter + 6;
 
     // process and type check arguments
     assume is#Vector(Dereference(__m, account));
-    assume IsValidReferenceParameter(__m, __frame, account);
+    assume IsValidReferenceParameter(__m, __local_counter, account);
     assume is#Vector(Dereference(__m, account));
     assume $DebugTrackLocal(11, 20, 0, 15265, Dereference(__m, account));
+
+    // increase the local counter
+    __local_counter := __local_counter + 6;
 
     // bytecode translation starts here
     call __t2 := CopyOrMoveRef(account);
@@ -4593,12 +4697,14 @@ requires ExistsTxnSenderAccount(__m, __txn);
     assume !__abort_flag;
     __saved_m := __m;
     __frame := __local_counter;
-    __local_counter := __local_counter + 4;
 
     // process and type check arguments
     assume is#Address(addr);
     __m := UpdateLocal(__m, __frame + 0, addr);
     assume $DebugTrackLocal(11, 21, 0, 15535, addr);
+
+    // increase the local counter
+    __local_counter := __local_counter + 4;
 
     // bytecode translation starts here
     call __tmp := CopyOrMoveValue(GetLocal(__m, __frame + 0));
@@ -4650,13 +4756,15 @@ requires ExistsTxnSenderAccount(__m, __txn);
     assume !__abort_flag;
     __saved_m := __m;
     __frame := __local_counter;
-    __local_counter := __local_counter + 4;
 
     // process and type check arguments
     assume is#Vector(Dereference(__m, account));
-    assume IsValidReferenceParameter(__m, __frame, account);
+    assume IsValidReferenceParameter(__m, __local_counter, account);
     assume is#Vector(Dereference(__m, account));
     assume $DebugTrackLocal(11, 22, 0, 15735, Dereference(__m, account));
+
+    // increase the local counter
+    __local_counter := __local_counter + 4;
 
     // bytecode translation starts here
     call __t1 := CopyOrMoveRef(account);
@@ -4698,12 +4806,14 @@ requires ExistsTxnSenderAccount(__m, __txn);
     assume !__abort_flag;
     __saved_m := __m;
     __frame := __local_counter;
-    __local_counter := __local_counter + 4;
 
     // process and type check arguments
     assume is#Address(addr);
     __m := UpdateLocal(__m, __frame + 0, addr);
     assume $DebugTrackLocal(11, 23, 0, 15901, addr);
+
+    // increase the local counter
+    __local_counter := __local_counter + 4;
 
     // bytecode translation starts here
     call __tmp := CopyOrMoveValue(GetLocal(__m, __frame + 0));
@@ -4756,12 +4866,14 @@ requires ExistsTxnSenderAccount(__m, __txn);
     assume !__abort_flag;
     __saved_m := __m;
     __frame := __local_counter;
-    __local_counter := __local_counter + 5;
 
     // process and type check arguments
     assume is#Address(addr);
     __m := UpdateLocal(__m, __frame + 0, addr);
     assume $DebugTrackLocal(11, 24, 0, 16132, addr);
+
+    // increase the local counter
+    __local_counter := __local_counter + 5;
 
     // bytecode translation starts here
     call __tmp := CopyOrMoveValue(GetLocal(__m, __frame + 0));
@@ -4811,12 +4923,14 @@ requires ExistsTxnSenderAccount(__m, __txn);
     assume !__abort_flag;
     __saved_m := __m;
     __frame := __local_counter;
-    __local_counter := __local_counter + 5;
 
     // process and type check arguments
     assume is#Address(addr);
     __m := UpdateLocal(__m, __frame + 0, addr);
     assume $DebugTrackLocal(11, 25, 0, 16385, addr);
+
+    // increase the local counter
+    __local_counter := __local_counter + 5;
 
     // bytecode translation starts here
     call __tmp := CopyOrMoveValue(GetLocal(__m, __frame + 0));
@@ -4864,13 +4978,15 @@ requires ExistsTxnSenderAccount(__m, __txn);
     assume !__abort_flag;
     __saved_m := __m;
     __frame := __local_counter;
-    __local_counter := __local_counter + 3;
 
     // process and type check arguments
     assume is#Vector(Dereference(__m, cap));
-    assume IsValidReferenceParameter(__m, __frame, cap);
+    assume IsValidReferenceParameter(__m, __local_counter, cap);
     assume is#Vector(Dereference(__m, cap));
     assume $DebugTrackLocal(11, 26, 0, 16640, Dereference(__m, cap));
+
+    // increase the local counter
+    __local_counter := __local_counter + 3;
 
     // bytecode translation starts here
     call __t1 := CopyOrMoveRef(cap);
@@ -4908,13 +5024,15 @@ requires ExistsTxnSenderAccount(__m, __txn);
     assume !__abort_flag;
     __saved_m := __m;
     __frame := __local_counter;
-    __local_counter := __local_counter + 3;
 
     // process and type check arguments
     assume is#Vector(Dereference(__m, cap));
-    assume IsValidReferenceParameter(__m, __frame, cap);
+    assume IsValidReferenceParameter(__m, __local_counter, cap);
     assume is#Vector(Dereference(__m, cap));
     assume $DebugTrackLocal(11, 27, 0, 16867, Dereference(__m, cap));
+
+    // increase the local counter
+    __local_counter := __local_counter + 3;
 
     // bytecode translation starts here
     call __t1 := CopyOrMoveRef(cap);
@@ -4952,12 +5070,14 @@ requires ExistsTxnSenderAccount(__m, __txn);
     assume !__abort_flag;
     __saved_m := __m;
     __frame := __local_counter;
-    __local_counter := __local_counter + 3;
 
     // process and type check arguments
     assume is#Address(check_addr);
     __m := UpdateLocal(__m, __frame + 0, check_addr);
     assume $DebugTrackLocal(11, 28, 0, 17057, check_addr);
+
+    // increase the local counter
+    __local_counter := __local_counter + 3;
 
     // bytecode translation starts here
     call __tmp := CopyOrMoveValue(GetLocal(__m, __frame + 0));
@@ -5044,7 +5164,6 @@ requires ExistsTxnSenderAccount(__m, __txn);
     assume !__abort_flag;
     __saved_m := __m;
     __frame := __local_counter;
-    __local_counter := __local_counter + 55;
 
     // process and type check arguments
     assume IsValidU64(txn_sequence_number);
@@ -5062,6 +5181,9 @@ requires ExistsTxnSenderAccount(__m, __txn);
     assume IsValidU64(txn_expiration_time);
     __m := UpdateLocal(__m, __frame + 4, txn_expiration_time);
     assume $DebugTrackLocal(11, 29, 4, 17457, txn_expiration_time);
+
+    // increase the local counter
+    __local_counter := __local_counter + 55;
 
     // bytecode translation starts here
     call __tmp := GetTxnSenderAddress();
@@ -5334,7 +5456,6 @@ requires ExistsTxnSenderAccount(__m, __txn);
     assume !__abort_flag;
     __saved_m := __m;
     __frame := __local_counter;
-    __local_counter := __local_counter + 37;
 
     // process and type check arguments
     assume IsValidU64(txn_sequence_number);
@@ -5349,6 +5470,9 @@ requires ExistsTxnSenderAccount(__m, __txn);
     assume IsValidU64(gas_units_remaining);
     __m := UpdateLocal(__m, __frame + 3, gas_units_remaining);
     assume $DebugTrackLocal(11, 30, 3, 19386, gas_units_remaining);
+
+    // increase the local counter
+    __local_counter := __local_counter + 37;
 
     // bytecode translation starts here
     call __tmp := GetTxnSenderAddress();
@@ -5536,16 +5660,18 @@ requires ExistsTxnSenderAccount(__m, __txn);
     assume !__abort_flag;
     __saved_m := __m;
     __frame := __local_counter;
-    __local_counter := __local_counter + 22;
 
     // process and type check arguments
     assume is#Vector(Dereference(__m, counter));
-    assume IsValidReferenceParameter(__m, __frame, counter);
+    assume IsValidReferenceParameter(__m, __local_counter, counter);
     assume is#Vector(Dereference(__m, counter));
     assume $DebugTrackLocal(11, 31, 0, 21344, Dereference(__m, counter));
     assume is#Address(sender);
     __m := UpdateLocal(__m, __frame + 1, sender);
     assume $DebugTrackLocal(11, 31, 1, 21344, sender);
+
+    // increase the local counter
+    __local_counter := __local_counter + 22;
 
     // bytecode translation starts here
     call __t6 := CopyOrMoveRef(counter);
@@ -5666,16 +5792,18 @@ requires ExistsTxnSenderAccount(__m, __txn);
     assume !__abort_flag;
     __saved_m := __m;
     __frame := __local_counter;
-    __local_counter := __local_counter + 7;
 
     // process and type check arguments
     assume is#Vector(Dereference(__m, counter));
-    assume IsValidReferenceParameter(__m, __frame, counter);
+    assume IsValidReferenceParameter(__m, __local_counter, counter);
     assume is#Vector(Dereference(__m, counter));
     assume $DebugTrackLocal(11, 32, 0, 22101, Dereference(__m, counter));
     assume is#Address(sender);
     __m := UpdateLocal(__m, __frame + 1, sender);
     assume $DebugTrackLocal(11, 32, 1, 22101, sender);
+
+    // increase the local counter
+    __local_counter := __local_counter + 7;
 
     // bytecode translation starts here
     call __tmp := LdConst(0);
@@ -5734,9 +5862,11 @@ requires ExistsTxnSenderAccount(__m, __txn);
     assume !__abort_flag;
     __saved_m := __m;
     __frame := __local_counter;
-    __local_counter := __local_counter + 8;
 
     // process and type check arguments
+
+    // increase the local counter
+    __local_counter := __local_counter + 8;
 
     // bytecode translation starts here
     call __tmp := GetTxnSenderAddress();
@@ -5812,15 +5942,17 @@ requires ExistsTxnSenderAccount(__m, __txn);
     assume !__abort_flag;
     __saved_m := __m;
     __frame := __local_counter;
-    __local_counter := __local_counter + 18;
 
     // process and type check arguments
     assume is#Vector(Dereference(__m, handle_ref));
-    assume IsValidReferenceParameter(__m, __frame, handle_ref);
+    assume IsValidReferenceParameter(__m, __local_counter, handle_ref);
     assume is#Vector(Dereference(__m, handle_ref));
     assume $DebugTrackLocal(11, 34, 0, 22958, Dereference(__m, handle_ref));
     __m := UpdateLocal(__m, __frame + 1, msg);
     assume $DebugTrackLocal(11, 34, 1, 22958, msg);
+
+    // increase the local counter
+    __local_counter := __local_counter + 18;
 
     // bytecode translation starts here
     call __t4 := CopyOrMoveRef(handle_ref);
@@ -5914,12 +6046,14 @@ requires ExistsTxnSenderAccount(__m, __txn);
     assume !__abort_flag;
     __saved_m := __m;
     __frame := __local_counter;
-    __local_counter := __local_counter + 6;
 
     // process and type check arguments
     assume is#Vector(handle);
     __m := UpdateLocal(__m, __frame + 0, handle);
     assume $DebugTrackLocal(11, 36, 0, 23597, handle);
+
+    // increase the local counter
+    __local_counter := __local_counter + 6;
 
     // bytecode translation starts here
     call __tmp := CopyOrMoveValue(GetLocal(__m, __frame + 0));
